basic proof outline stated

FundThm.v
@@ -1,13 +1,32 @@
 
+Require Import Program.
 Require Import Arith.
 Require Import List.
 Import ListNotations.
 Require Import SnocList.
-Require Import Relations.Relation_Operators.
+Require Import Relations.
 
 Require Import JRWTactics.
 
 Set Implicit Arguments.
+
+
+Inductive fin : nat -> Set :=
+  | FO : forall n, fin (S n)
+  | FS : forall n, fin n -> fin (S n).
+
+Check (FS (FO 4)).
+
+Check (FS (FS (FO 3))).
+
+Check FO.
+
+Lemma fin_eq_dec :
+  forall n (a b : fin n), 
+    {a = b} + {a <> b}.
+Proof.
+  admit.
+Qed.
 
 
 Class alphabet :=
@@ -16,13 +35,172 @@ Class alphabet :=
     letter : Type;
     default : letter;
     letter_eq_dec : forall (l l' : letter), {l = l'} + {l <> l'};
-    sle : letter -> letter -> Prop;
-    slt : letter -> letter -> Prop; (* need to restrain this *)
-    total_ord : forall (x y : letter), {sle x y} + {~(sle x y)}
+    ale : letter -> letter -> Prop;
+    alt : letter -> letter -> Prop; (* need to restrain this *)
+    total_ord : forall (x y : letter), {ale x y} + {~(ale x y)}
     (* reflexivity *)
     (* transitivity *)
+    (* bijection between letters and fin types *)
   }.
 
+
+Section Word.
+  Context `{ sigma : alphabet }.
+
+  Definition word := snoclist letter.
+
+  Inductive rotate_by_one : word -> word -> Prop :=
+    | RBO_step : forall (a : letter) (w : snoclist letter),
+                   rotate_by_one (snoc w a) ([a] +++ w).
+
+  Definition rotation_of : word -> word -> Prop :=
+    clos_refl_trans word rotate_by_one.
+  
+  Lemma rotation_of__same_length :
+    forall w w',
+      rotation_of w w' ->
+      length w = length w'.
+  Proof.
+    admit.
+  Qed.
+
+  Inductive wlt : word -> word -> Prop :=
+    | wlt_snil : forall a w,
+                   wlt snil (snoc w a)
+    | wlt_alt  : forall a a' w w',
+                   alt a a' ->
+                   wlt ([a] +++ w) ([a'] +++ w')
+    | wlt_aeq  : forall a a' w w',
+                   a = a' ->
+                   wlt w w' ->
+                   wlt ([a] +++ w) ([a'] +++ w').
+
+  Definition wle (w w' : word) : Prop :=
+    (w = w') \/ (wlt w w').
+
+  Inductive prefix : word -> word -> Prop :=
+    | P_refl : forall w, 
+                 prefix w w
+    | P_snoc : forall w w' a, 
+                 prefix w w' ->
+                 prefix w (w' ::: a).
+
+  Fixpoint all_prefixes (w : word) : snoclist word :=
+    match w with
+      | snil      => [snil]
+      | snoc w' a => snoc (all_prefixes w') w
+    end.
+
+  Fixpoint concat_n (n : nat) (w : word) :=
+    match n with
+      | O => snil
+      | S n' => w +++ (concat_n n' w)
+    end.
+
+  Definition periodic (w : word) : Prop :=
+    exists w',
+      length w' < length w /\
+      exists n,
+        concat_n n w' = w.
+
+End Word.
+
+
+Section FundThm.
+  Context `{ sigma : alphabet }.
+  
+  Definition necklace (w : word) : Prop :=
+    forall w',
+      rotation_of w' w ->
+      wle w w'.
+
+  Definition prenecklace (w : word) : Prop :=
+    exists w',
+      necklace (w +++ w').
+
+  Definition lyndon (w : word) : Prop :=
+    necklace w /\ ~(periodic w).
+
+  Hint Unfold necklace.
+  Hint Unfold prenecklace.
+  Hint Unfold lyndon.
+
+  Lemma lyndon_dec :
+    forall w,
+      {lyndon w} + {~(lyndon w)}.
+  Proof.
+    admit.
+  Qed.
+
+  (* lyn prefixes are ordered from smallest to largest *)
+  Definition lyn_prefixes (w : word) : snoclist word :=
+    sfilter (fun p => if (lyndon_dec p) then true else false) (all_prefixes w).
+
+  (* lyn takes size of last element of lyn_prefixes *)
+  Definition lyn (w : word) : nat :=
+    match lyn_prefixes w with
+      | snil => 0
+      | l:::a => length a
+    end.
+
+  Lemma concat_n_necklace :
+    forall w n,
+      necklace w ->
+      1 <= n ->
+      necklace (concat_n n w).
+  Proof.
+    admit.
+  Qed.
+
+  Lemma prenecklace_characterization_1 :
+    forall w,
+      prenecklace w <->
+      (forall i,
+         i <= length w ->
+         wle (first_n i w) (last_n i w)).
+  Proof.
+    admit.
+  Qed.
+
+  Lemma prenecklace_characterization_2 : 
+    forall w i,
+      i <= length w ->
+      i > lyn w ->
+      nth default i w = nth default (i - lyn w) w.
+  Proof.
+    admit.
+  Qed.
+
+  Lemma lyndon_characterization :
+    forall w,
+      lyndon w <->
+      (forall x y,
+         w = x+++y ->
+         wlt (y+++x) w).
+  Proof.
+    admit.
+  Qed.
+
+  Lemma next_lyn : 
+    forall w a,
+      lyn (snoc w a) = lyn w \/ lyn (snoc w a) = length w + 1.
+  Proof.
+    admit.
+  Qed.
+
+  Theorem fund_thm_of_necklaces :
+    forall w p,
+      prenecklace w ->
+      p = lyn w ->
+      forall b,
+        (prenecklace (snoc w b) <-> ale (nth_from_end default p w) b) /\
+        (b = nth_from_end default p w -> lyn (snoc w b) = p) /\
+        (alt (nth_from_end default p w) b -> lyn (snoc w b) = length w + 1).
+  Proof.
+    admit.
+  Qed.
+
+  
 
 (*
 To Do:
@@ -42,327 +220,6 @@ To Do:
 
 *)
 
-
-Section FundThm.
-  Context `{ sigma : alphabet }.
-
-  Definition word := snoclist letter.
-  
-  Inductive rotate_by_one : word -> word -> Prop :=
-    | RBO_step : forall (a : letter) (w : snoclist letter),
-                   rotate_by_one (snoc w a) ([a] +++ w).
-
-  Definition rotation_of : word -> word -> Prop :=
-    clos_refl_trans word rotate_by_one.
-  
-  Lemma rotation_of__same_length :
-    forall w w',
-      rotation_of w w' ->
-      length w = length w'.
-  Proof.
-    admit.
-  Qed.
-
-  Inductive wle : word -> word -> Prop :=
-    | wle_nil : wle snil snil
-    | wle_snoc : forall a a' w w',
-                   a = a' ->
-                   wle w w' ->
-                   wle (w ::: a) ([a'] +++ w').
-
-  Definition lex_smallest (w : word) : Prop :=
-    forall w',
-      rotation_of w' w ->
-      wle w w'.
-
-  Definition necklace (w : word) : Prop := 
-    lex_smallest w.
-
-  Definition prenecklace (w : word) : Prop :=
-    exists w',
-      necklace (w +++ w').
-
-  Fixpoint concat_n (n : nat) (w : word) :=
-    match n with
-      | O => snil
-      | S n' => w +++ (concat_n n' w)
-    end.
-
-  Definition periodic (w : word) : Prop :=
-    exists w',
-      length w' < length w /\
-      exists n,
-        concat_n n w' = w.
-
-  Definition lyndon (w : word) : Prop :=
-    necklace w /\ ~(periodic w).
-
-  Lemma lyndon_dec :
-    forall w,
-      {lyndon w} + {~(lyndon w)}.
-  Proof.
-    admit.
-  Qed.
-
-  Inductive prefix : word -> word -> Prop :=
-    | P_refl : forall w, 
-                 prefix w w
-    | P_snoc : forall w w' a, 
-                 prefix w w' ->
-                 prefix w (w' ::: a).
-
-  Fixpoint all_prefixes (w : word) : snoclist word :=
-    match w with
-      | snil => snil
-      | snoc w' a => smap (fun l => snoc l a) (all_prefixes w')
-    end.
-
-  Definition lyn_prefixes (w : word) : snoclist word :=
-    sfilter (fun p => if (lyndon_dec p) then true else false) (all_prefixes w).
-
-  Definition lyn (w : word) : nat :=
-    match lyn_prefixes w with
-      | snil => 0
-      | l:::a => length a
-    end.
-
-  Lemma concat_n_necklace :
-    forall w n,
-      necklace w ->
-      1 <= n ->
-      necklace (concat_n n w).
-  Proof.
-    admit.
-  Qed.
-
-
-  Theorem fund_thm_of_necklaces :
-    forall w n p,
-      length w = n - 1 ->
-      prenecklace w ->
-      p = lyn w ->
-      forall b,
-        (prenecklace (snoc w b) <-> sle (nth_from_end p w default) b) /\
-        (b = nth_from_end p w default -> lyn (snoc w b) = p) /\
-        (slt (nth_from_end p w default) b -> lyn (snoc w b) = n).
-  Proof.
-    admit.
-  Qed.
-
-End FundThm.
-
-
-(*
-Section FundThm'.
-  Context `{ sigma : alphabet }.
-
-  Definition word := list letter.
-
-  Inductive rotate_by_one : word -> word -> Prop :=
-    | RBO_step : forall a w, rotate_by_one (w++[a]) (a :: w).
-
-  Definition rotation_of : word -> word -> Prop :=
-    clos_refl_trans word rotate_by_one.
-
-  Lemma rotation_of__same_length :
-    forall w w',
-      rotation_of w w' ->
-      length w = length w'.
-  Proof.
-    admit.
-  Qed.
-
-  Inductive wle : word -> word -> Prop :=
-    | wle_nil : wle nil nil
-    | wle_cons : forall a a' w w',
-                   a = a' ->
-                   wle w w' ->
-                   wle (a :: w) (a' :: w').
-
-  Definition lex_smallest (w : word) : Prop :=
-    forall w',
-      rotation_of w' w ->
-      wle w w'.
-
-  Definition necklace (w : word) : Prop := 
-    lex_smallest w.
-
-  Definition prenecklace (w : word) : Prop :=
-    exists w',
-      necklace (w ++ w').
-
-  Fixpoint concat (n : nat) (w : word) :=
-    match n with
-      | O => nil
-      | S n' => w ++ (concat n' w)
-    end.
-
-  Definition periodic (w : word) : Prop :=
-    exists w',
-      length w' <= length w /\
-      exists n,
-        concat n w' = w.
-
-  Definition lyndon (w : word) : Prop :=
-    necklace w /\ ~(periodic w).
-
-  Inductive prefix : word -> word -> Prop :=
-    | P_refl : forall w, 
-                 prefix w w
-    | P_snoc : forall w w' a, 
-                 prefix w w' ->
-                 prefix w (w' ++ [a]).
-
-  Fixpoint all_prefixes (w : word) : list word :=
-    let w' = rev w in
-    match w' with
-      | nil => 
-
-
-  (* define *set* of lyndon prefixes for a given word,
-     then define lyn as the length of the longest one *)
-
-  Definition longest_lyn_prefix (p w : word) : Prop :=
-    prefix p w /\
-    lyndon p /\
-    (forall p',
-       prefix p' w ->
-       lyndon p' ->
-       length p' < length p).
-
-  Definition lyn (w : word) : nat :=
-    
-
-
-(*
-Let \alpha = a_1 a_2 ... a_{n-1} \in P_k(n-1) and let p = lyn(\alpha).
-The string \alpha b \in P_k(n) iff a_{n-p} \le b \le k-1.  Furthermore,
-
-lyn(\alpha b) = 
-  | p     if b = a_{n-p}
-  | n     else.
-*)
-
-
-
-  Definition lyn (w : word) : Prop :=
-    
-    
-  Theorem fundamental_theorem :
-    
-
-(*
-  Inductive rotation_of {n : nat} : word n -> word n -> Prop :=
-    | RO_refl : forall w, 
-                  rotation_of w w
-    | RO_step : forall {n' : nat} (a : letter) (w' : word n') (w : word (S n')), 
-                  rotation_of (append w' [a]) w ->
-                  rotation_of (a :: w') w.
-*)
-
-
-End FundThm.
-
-
-
-
-(*
-Inductive fin : nat -> Set :=
-  | FO : forall {n}, fin (S n)
-  | FS : forall {n}, fin n -> fin (S n).
-
-Check (FS (FO)).
-
-Check FO.
-
-Lemma fin_eq_dec :
-  forall n (a b : fin n), 
-    {a = b} + {a <> b}.
-Proof.
-  admit.
-Qed.
-
-
-
-Section FundThm'.
-
-Variable k : nat.
-
-Definition sigma := fin (S k).
-Hint Unfold sigma.
-
-
-Fixpoint fin_to_nat {n : nat} (a : fin n) :=
-  match a with
-    | FO m => m
-    | FS n' a' => fin_to_nat a'
-  end.
-
-Definition sle' (a b : sigma) := le (fin_to_nat a) (fin_to_nat b).
-
-(*
-Reserved Notation "a '<<==' b" (at level 70).
-
-Inductive sle (a : sigma) : sigma -> Prop :=
-  | sle_n : a <<== a
-  | sle_S : forall b, a <<== b -> a <<== b
-
-where "a '<<==' b" := (sle a b).
-*)
-
-Print le.
-
-(*
-Inductive sle'' {n : nat} (a : fin n) : fin n -> Prop :=
-  | sle_a : sle'' a a
-  | sle_S : forall b, sle'' a b -> sle'' a (FS b)
-*)
-
-Inductive sle'' : forall n, fin (S n) -> fin (S n) -> Prop :=
-  | sle_O : forall n b, sle'' n FO b
-  | sle_S : forall n a b, sle'' n a b -> sle'' (S n) (FS a) (FS b).
-
-
-
-
-  | sle'_n : forall a, sle' a a
-  | 
-
-
-Fixpoint sleb (n : nat) (a b : fin n) : bool :=
-  match a with
-    | FO _ => true
-    | FS n' a' => match b with
-                    | FO _ => false
-                    | FS n' b' => sleb n' a' b'
-                  end
-  end.
-
-
-
-Definition word (n : nat) := t sigma n. (* t is the vector type constructor *)
-
-
-End FundThm.  
-*)
-
-
-
-
-
-
-(* Fundamental Theorem of Necklaces *)
-
-(* 
-Let \alpha = a_1 a_2 ... a_{n-1} \in P_k(n-1) and let p = lyn(\alpha).
-The string \alpha b \in P_k(n) iff a_{n-p} \le b \le k-1.  Furthermore,
-
-lyn(\alpha b) = 
-  | p     if b = a_{n-p}
-  | n     else.
-*)
-
-*)
 
 
 
